\section{\Large Exercise 2.13:}If $\ket{w}$ and $\ket{v}$ are any two vectors,
show that $(\ket{w}\bra{v})^\dagger = \ket{v}\bra{w}$.
\newline
{\large proof:}
Suppose $\ket{\psi},\ \ket{\phi}$ are arbitrary vectors in $V$. 
\begin{align*}
        \left(\ket{\psi},\ (\ket{w}\bra{v}) \ket{\phi}\right)^* &=
        \left((\ket{w}\bra{v})^\dagger \ket{\psi},\  \ket{\phi}\right)^*\\
        &= \left(\ket{\phi},\ (\ket{w}\bra{v})^\dagger \ket{\psi} \right)\\
        &= \bra{\phi} (\ket{w}\bra{v})^\dagger \ket{\psi}.
\end{align*}
On the other hand,
\begin{align*}
        \left(\ket{\psi},\ (\ket{w}\bra{v}) \ket{\phi}\right)^*
        &= (\braket{\psi | w} \braket{v | \phi})^*\\
        &= \braket{\phi | v} \braket{w | \psi}.
\end{align*}

Thus
\begin{align*}
        \bra{\phi} (\ket{w}\bra{v})^\dagger \ket{\psi} = \braket{\phi | v} \braket{w | \psi} \text{ for arbitrary vectors } \ket{\psi},\ \ket{\phi}\\
        \therefore (\ket{w}\bra{v})^\dagger = \ket{v}\bra{w}
\end{align*}
(\hyperlink{hukushuu3.5}{復習3.5}による。)
